

# Linear Algebra

Qing-Jie Yuan

December 8, 2025

## Contents

<b>1</b>	<b>Formalism</b>	<b>1</b>
<b>2</b>	<b>Simple Systems</b>	<b>1</b>
2.1	Harmonic Oscillator . . . . .	1
2.2	Landau Level . . . . .	4
2.2.1	Landau Gauge . . . . .	5
2.2.2	Symmetric Gauge . . . . .	5
<b>3</b>	<b>Angular Momentum</b>	<b>6</b>
<b>4</b>	<b>Central Potential</b>	<b>6</b>
<b>5</b>	<b>Approximation Methods</b>	<b>6</b>
<b>6</b>	<b>Scattering Theory</b>	<b>6</b>

## 1 Formalism

## 2 Simple Systems

### 2.1 Harmonic Oscillator

The Hamiltonian for one-dimensional harmonic oscillator is

$$H = \frac{1}{2m}p^2 + \frac{m\omega^2}{2}q^2. \quad (2.1)$$

We define

$$a = \frac{1}{\sqrt{2\hbar}}\left(\sqrt{m\omega}q + i\frac{p}{\sqrt{m\omega}}\right) \text{ and } a^\dagger = \frac{1}{\sqrt{2\hbar}}\left(\sqrt{m\omega}q - i\frac{p}{\sqrt{m\omega}}\right). \quad (2.2)$$

We can get

$$H = \hbar\omega\left(a^\dagger a + \frac{1}{2}\right) \quad (2.3)$$

and

$$[a, a^\dagger] = 1. \quad (2.4)$$

There is a long discussion to get the spectrum of this Hamiltonian...

The result is

$$E_n = \hbar\omega\left(n + \frac{1}{2}\right); \quad n = 0, 1, 2, \dots \quad (2.5)$$

We define

$$x = \sqrt{\frac{m\omega}{\hbar}}q. \quad (2.6)$$

Then

$$dx = \text{ and } \frac{d}{dx} = \sqrt{\frac{\hbar}{m\omega}} \frac{d}{dq} = i\sqrt{\frac{1}{m\hbar\omega}}p. \quad (2.7)$$

The creation and annihilation operators in the  $x$ -representation are

$$a = \frac{1}{\sqrt{2}}\left(x + \frac{d}{dx}\right); \quad a^\dagger = \frac{1}{\sqrt{2}}\left(x - \frac{d}{dx}\right). \quad (2.8)$$

The lowest eigenstate is got by the equation

$$\left(x + \frac{d}{dx}\right)\varphi_0(x) = 0 \quad (2.9)$$

the general solution is given by

$$\varphi_0(x) = c_0 \exp\left(-\frac{x^2}{2}\right), \quad (2.10)$$

we can choose  $c_0$  from the normalization condition

$$1 \stackrel{!}{=} \int_{-\infty}^{+\infty} dq |\varphi_0(q)|^2 = \sqrt{\frac{\hbar}{m\omega}} |c_0|^2 \int_{-\infty}^{+\infty} dx e^{-x^2} = \sqrt{\frac{\pi\hbar}{m\omega}} |c_0|^2 \quad (2.11)$$

as  $c_0 = \left(\frac{m\omega}{\hbar\pi}\right)^{1/4}$ , and higher eigenwavefunctions can be got from

$$\begin{aligned} \varphi_n(x) = \langle x|n\rangle &= \frac{1}{\sqrt{n!}} \langle x|(a^\dagger)^n|0\rangle = \frac{1}{\sqrt{2^n n!}} \left(x - \frac{d}{dx}\right)^n \varphi_0(x) \\ &= \frac{1}{\sqrt{2^n n!}} \left(\frac{m\omega}{\hbar\pi}\right)^{1/4} \left(x - \frac{d}{dx}\right)^n \exp\left(-\frac{x^2}{2}\right). \end{aligned} \quad (2.12)$$

The equation can be converted to the definition of the Hermite polynomials  $H_n(x)$ . The relation

is given by

$$\varphi_n(x) = \frac{1}{\sqrt{2^n n!}} \left( \frac{m\omega}{\hbar\pi} \right)^{1/4} \exp\left(-\frac{x^2}{2}\right) H_n(x) \quad (2.13)$$

From (2.12), we get

$$H_n(x) = \exp\left(\frac{x^2}{2}\right) \left(x - \frac{d}{dx}\right)^n \exp\left(-\frac{x^2}{2}\right), \quad (2.14)$$

which is equivalent to the definition of the Hermite polynomials:

$$H_n(x) = (-1)^n e^{x^2} \frac{d^n}{dx^n} e^{-x^2}. \quad (2.15)$$

The equivalence can be seen by

$$\begin{aligned} (-1)^n \exp(x^2) \frac{d^n}{dx^n} \exp(-x^2) &= (-1)^n e^{x^2} \frac{d}{dx} e^{-x^2} e^{x^2} \frac{d}{dx} e^{-x^2} \dots e^{x^2} \frac{d}{dx} e^{-x^2} \\ &= (-1)^n \left[ e^{x^2} \frac{d}{dx} e^{-x^2} \right]^n \\ &= (-1)^n \left[ e^{\frac{x^2}{2}} e^{\frac{x^2}{2}} \frac{d}{dx} e^{-\frac{x^2}{2}} e^{-\frac{x^2}{2}} \right]^n \\ &= (-1)^n \left[ e^{\frac{x^2}{2}} \left( \frac{d}{dx} - x \right) e^{-\frac{x^2}{2}} \right]^n \\ &= e^{\frac{x^2}{2}} \left( x - \frac{d}{dx} \right) e^{-\frac{x^2}{2}} e^{\frac{x^2}{2}} \left( x - \frac{d}{dx} \right) e^{-\frac{x^2}{2}} \dots e^{\frac{x^2}{2}} \left( x - \frac{d}{dx} \right) e^{-\frac{x^2}{2}} \\ &= e^{\frac{x^2}{2}} \left( x - \frac{d}{dx} \right)^n e^{-\frac{x^2}{2}}. \end{aligned} \quad (2.16)$$

The only non-trivial step is the operator relation

$$\frac{1}{f(x)} \frac{d}{dx} f(x) = \frac{d}{dx} + \frac{f'(x)}{f(x)}. \quad (2.17)$$

Now we give the general solution of the one-dimensional harmonic oscillator, which may have a non-trivial displacement  $d$  from the original point,

$$\varphi_n(q) = \frac{1}{\sqrt{2^n n!}} \left( \frac{m\omega}{\hbar\pi} \right)^{1/4} \exp\left(-\frac{(q+d)^2}{2l_\omega^2}\right) H_n\left(\frac{q+d}{l_\omega}\right), \quad (2.18)$$

where  $l_\omega \equiv \sqrt{\frac{\hbar}{m\omega}}$ .

## 2.2 Landau Level

The Lagrangian for a particle of charge  $-e$  and mass  $m$  moving in a magnetic vector potential is

$$L = \frac{1}{2}m\dot{\mathbf{x}}^2 - e\dot{\mathbf{x}} \cdot \mathbf{A}. \quad (2.19)$$

The canonical momentum is

$$\mathbf{p} = m\dot{\mathbf{x}} - e\mathbf{A}. \quad (2.20)$$

The Hamiltonian is

$$H = \dot{\mathbf{x}} \cdot \mathbf{p} - L = \frac{1}{2m}(\mathbf{p} + e\mathbf{A})^2. \quad (2.21)$$

Define

$$\pi \equiv \mathbf{p} + e\mathbf{A} = m\dot{\mathbf{x}}. \quad (2.22)$$

Poisson brackets are

$$\{x_i, p_j\} = \delta_{ij} \text{ and } \{x_i, x_j\} = \{p_i, p_j\} = 0. \quad (2.23)$$

We can get

$$\{\pi_i, \pi_j\} = \sum_{k=1}^3 \frac{\partial \pi_i}{\partial x_k} \frac{\partial \pi_j}{\partial p_k} - \frac{\partial \pi_i}{\partial p_k} \frac{\partial \pi_j}{\partial x_k} = -e\epsilon_{ijk}B_k. \quad (2.24)$$

The quantization is given by

$$[x_i, p_j] = i\hbar\delta_{ij} \text{ and } [x_i, x_j] = [p_i, p_j] = 0. \quad (2.25)$$

The particle is constrained in the  $x$ - $y$  plane and the magnetic field is set to  $\nabla \times \mathbf{A} = B\hat{\mathbf{z}}$ , the Hamiltonian is

$$H = \frac{1}{2m}(\pi_x^2 + \pi_y^2), \quad (2.26)$$

and we have<sup>1</sup>

$$[\pi_x, \pi_y] = -ie\hbar B. \quad (2.27)$$

If we define

$$a = \frac{1}{\sqrt{2e\hbar B}}(\pi_x - i\pi_y) \text{ and } a^\dagger = \frac{1}{\sqrt{2e\hbar B}}(\pi_x + i\pi_y), \quad (2.28)$$

we have

$$[a, a^\dagger] = 1 \quad (2.29)$$

Now the Hamiltonian is

$$H = \hbar\omega_B \left( a^\dagger a + \frac{1}{2} \right), \quad (2.30)$$

---

<sup>1</sup>We can see if we set  $p = -\pi_y$  and  $q = \pi_x/eB$ , the Hamiltonian and commutator is just the same as that of the harmonic oscillator.

where  $\omega_B \equiv eB/m$ . This Hamiltonian has the same algebraic structure as the that of harmonic. Thus we have the spectrum

$$E_n = \hbar\omega_B \left( n + \frac{1}{2} \right), \quad (2.31)$$

which is called the Landau level. Then we compute the eigenstates in two gauges respectively.

### 2.2.1 Landau Gauge

The Landau gauge is the choice

$$\mathbf{A} = xB\hat{\mathbf{y}}. \quad (2.32)$$

Now the Hamiltonian is

$$H = \frac{1}{2m}p_x^2 + \frac{1}{2}m\omega_B^2 \left( x + \frac{p_y}{eB} \right)^2. \quad (2.33)$$

There exists translation invariance in  $y$  direction, meaning  $[p_y, H] = 0$ , which tells us  $p_y$  eigenvalues are good quantum number to characterize states. We can use the ansatz

$$\psi_k(x, y) = e^{iky} f_k(x). \quad (2.34)$$

Apply the Hamiltonian to this state, we get

$$H\psi_k(x, y) = \left[ \frac{1}{2m}p_x^2 + \frac{1}{2}m\omega_B^2 \left( x + \frac{\hbar k}{eB} \right)^2 \right] \psi_k(x, y) \equiv e^{iky} H_k f_k(x), \quad (2.35)$$

where  $H_k$  can be interpreted as a harmonic oscillator with a displacement. By using the result (2.18), we get

$$\psi_k(x, y) \sim e^{iky} H_n \left( \frac{x + kl_B^2}{l_b} \right) e^{-(x+kl_B^2)^2/2l_B^2} \quad (2.36)$$

where  $l_B = \sqrt{\frac{\hbar}{m\omega_B}} = \sqrt{\frac{\hbar}{eB}}$ .

### 2.2.2 Symmetric Gauge

The symmetric gauge is

$$\mathbf{A} = -\frac{yB}{2}\hat{\mathbf{x}} + \frac{xB}{2}\hat{\mathbf{y}}. \quad (2.37)$$

We have rotational symmetry about the origin in this choice of gauge, which means the angular momentum is a good quantum number.

**3 Angular Momentum**

**4 Central Potential**

**5 Approximation Methods**

**6 Scattering Theory**